From the definition:
$$\left( {n^2 - n + 1}\right) + \left( {n^2 - n + 3}\right) + \ldots + \left( {n^2 + n - 1}\right)$$

can be written:
$$\left( {n^2 - n + 1}\right) + \left( {n^2 - n + 3}\right) + \ldots + \left( {n^2 - n + 2 n - 1}\right)$$

Writing this in sum notation:

$$\left( {n^2 - n + 1}\right) + \left( {n^2 - n + 3}\right) + \ldots + \left( {n^2 - n + 2 n - 1}\right)$$
$$ = \sum_{k  = 1}^n \left( {n^2 - n + 2 k - 1}\right)$$
$$ = n \left( {n^2 - n}\right) + \sum_{k  = 1}^n \left( {2 k - 1}\right)$$
$$ = n^3 - n^2 + n^2 \text{\quad Odd Number Theorem}$$
$$ = n^3$$

$\blacksquare$